@base <http://linked.data.gov.au/def/ont/iso19160-1-address/Address/code/> .
@prefix dc: <http://purl.org/dc/elements/1.1/> .
@prefix dct: <http://purl.org/dc/terms/> .
@prefix dct: <http://purl.org/dc/terms/> .
@prefix owl: <http://www.w3.org/2002/07/owl#> .
@prefix rdf: <http://www.w3.org/1999/02/22-rdf-syntax-ns#> .
@prefix rdfs: <http://www.w3.org/2000/01/rdf-schema#> .
@prefix sdo: <https://schema.org/> .
@prefix skos: <http://www.w3.org/2004/02/skos/core#> .
@prefix xsd: <http://www.w3.org/2001/XMLSchema#> .

<AddressAliasTypeCollection> a skos:Collection ;
    skos:member <AddressAliasType/classAlias>,
        <AddressAliasType/colloquialAlias>,
        <AddressAliasType/lifecycleAlias>,
        <AddressAliasType/localeAlias>,
        <AddressAliasType/unspecifiedAlias> ;
    skos:prefLabel "Address Alias Type - Collection" .

<AddressClass> a skos:ConceptScheme ;
    skos:prefLabel "AddressClass - ConceptScheme" .

<AddressClassCollection> a skos:Collection ;
    skos:prefLabel "Address Class - Collection" .

<AddressCodelist> a owl:Ontology , skos:ConceptScheme ;
    rdfs:label "ISO19160-1:2015 Address Codelist"@en ;
    dct:contributor [ 
      a sdo:Person ;
      sdo:affiliation [
        a sdo:Organization ;
        sdo:url <https://surroundaustralia.com> ;
        sdo:name "SURROUND Australia Pty Ltd" ;      
      ] ;
      sdo:email <mailto:nicholas.car@surroundaustralia.com> ;
      sdo:identifier <https://orcid.org/0000-0002-8742-7730> ;
      sdo:name "Nicholas J. Car"
    ] ;  
    dct:creator [
      a sdo:Organization ;
      sdo:name "ISO TC211, Group for Ontology Management" ;
      sdo:url <https://def.isotc211.org/> ;
    ] ;
    dct:created "2017-12-01"^^xsd:date ;
    dct:description "A SKOS vocabulary version of the ISO19160-1:2015 standard's codelists. In addition to SKOS vocabulary formulation, each specialised ConceptSceme's members are typed according to an OWL class."@en ;
    rdfs:comment "A SKOS vocabulary version of the ISO19160-1:2015 standard's codelists. In addition to SKOS vocabulary formulation, each specialised ConceptSceme's members are typed according to an OWL class."@en ;
    dct:issued "2017-12-01" ;
    dct:modified "2019-10-24"^^xsd:date ;
    dct:publisher [
      a sdo:Organization ;
      sdo:identifier <http://linked.data.gov.au/org/agldwg> ;
      sdo:name "Australian Government Linked Data Working Group" ;
    ] ;
    dct:title "ISO19160-1 Address Codelist"@en ;
    owl:versionInfo "v1.1" ;
    skos:hasTopConcept
        <AddressAliasType/classAlias>,
        <AddressAliasType/colloquialAlias>,
        <AddressAliasType/lifecycleAlias>,
        <AddressAliasType/localeAlias>,
        <AddressAliasType/unspecifiedAlias>,
        <AddressComponentType/addressedObjectIdentifier>,
        <AddressComponentType/administrativeAreaName>,
        <AddressComponentType/countryCode>,
        <AddressComponentType/countryName>,
        <AddressComponentType/localityName>,
        <AddressComponentType/postOfficeName>,
        <AddressComponentType/postcode>,
        <AddressComponentType/thoroughfareName>,
        <AddressComponentValueType/abbreviatedAlternative>,
        <AddressComponentValueType/colloquialAlternative>,
        <AddressComponentValueType/defaultValue>,
        <AddressComponentValueType/lifecycleAlternative>,
        <AddressComponentValueType/localeAlternative>,
        <AddressLifecycleStage/current>,
        <AddressLifecycleStage/proposed>,
        <AddressLifecycleStage/rejected>,
        <AddressLifecycleStage/reserved>,
        <AddressLifecycleStage/retired>,
        <AddressLifecycleStage/unknown>,
        <AddressStatus/official>,
        <AddressStatus/unknown>,
        <AddressStatus/unofficial>,
        <AddressTypology/area>,
        <AddressTypology/service>,
        <AddressTypology/thoroughfare>,
        <AddressableObjectLifecycleStage/approved>,
        <AddressableObjectLifecycleStage/ceasedToExist>,
        <AddressableObjectLifecycleStage/exists>,
        <AddressableObjectLifecycleStage/proposed>,
        <AddressableObjectLifecycleStage/underConstruction>,
        <AddressableObjectLifecycleStage/unknown> .

<AddressComponentTypeCollection> a skos:Collection ;
    skos:member
        <AddressComponentType/addressedObjectIdentifier>,
        <AddressComponentType/administrativeAreaName>,
        <AddressComponentType/countryCode>,
        <AddressComponentType/countryName>,
        <AddressComponentType/localityName>,
        <AddressComponentType/postOfficeName>,
        <AddressComponentType/postcode>,
        <AddressComponentType/thoroughfareName> ;
    skos:prefLabel "Address Component Type - Collection" .

<AddressComponentValueTypeCollection> a skos:Collection ;
    skos:member
        <AddressComponentValueType/abbreviatedAlternative>,
        <AddressComponentValueType/colloquialAlternative>,
        <AddressComponentValueType/defaultValue>,
        <AddressComponentValueType/lifecycleAlternative>,
        <AddressComponentValueType/localeAlternative> ;
    skos:prefLabel "Address Component Value Type - Collection" .

<AddressLifecycleStageCollection> a skos:Collection ;
    skos:member
        <AddressLifecycleStage/current>,
        <AddressLifecycleStage/proposed>,
        <AddressLifecycleStage/rejected>,
        <AddressLifecycleStage/reserved>,
        <AddressLifecycleStage/retired>,
        <AddressLifecycleStage/unknown> ;
    skos:prefLabel "AddressLifecycleStage - Collection" .

<AddressPositionType> a skos:ConceptScheme ;
    skos:prefLabel "Address Position Type - ConceptScheme" .

<AddressPositionTypeCollection> a skos:Collection ;
    skos:prefLabel "Address Position Type - Collection" .

<AddressStatusCollection> a skos:Collection ;
    skos:member <AddressStatus/official>,
        <AddressStatus/unknown>,
        <AddressStatus/unofficial> ;
    skos:prefLabel "Address Status - Collection" .

<AddressTypologyCollection> a skos:Collection ;
    skos:member <AddressTypology/area>,
        <AddressTypology/service>,
        <AddressTypology/thoroughfare> ;
    skos:prefLabel "Address Typology - Collection" .

<AddressableObjectLifecycleStageCollection> a skos:Collection ;
    skos:member <AddressableObjectLifecycleStage/approved>,
        <AddressableObjectLifecycleStage/ceasedToExist>,
        <AddressableObjectLifecycleStage/exists>,
        <AddressableObjectLifecycleStage/proposed>,
        <AddressableObjectLifecycleStage/underConstruction>,
        <AddressableObjectLifecycleStage/unknown> ;
    skos:prefLabel "Addressable Object Lifecycle Stage - Collection" .

<AddressableObjectType> a skos:ConceptScheme ;
    skos:prefLabel "Addressable Object Type - ConceptScheme" .

<AddressableObjectTypeCollection> a skos:Collection ;
    skos:prefLabel "Addressable Object Type - Collection" .

<ReferenceObjectType> a skos:ConceptScheme ;
    skos:prefLabel "Reference Object Type - ConceptScheme" .

<ReferenceObjectTypeCollection> a skos:Collection ;
    skos:prefLabel "Reference Object Type - Collection" .

<AddressAliasType/classAlias> a <AddressAliasType>,
        skos:Concept , owl:NamedIndividual ;
    skos:definition "The address alias is from a different address class." ;
		rdfs:comment "The address alias is from a different address class." ;
    skos:inScheme <AddressAliasType> ;
    skos:prefLabel "Class Alias" .

<AddressAliasType/colloquialAlias> a <AddressAliasType>,
        skos:Concept , owl:NamedIndividual ;
    skos:definition "The address alias is a colloquial version of the address." ;
		rdfs:comment "The address alias is a colloquial version of the address." ;
    skos:inScheme <AddressAliasType> ;
    skos:prefLabel "Colloquial Alias" .

<AddressAliasType/lifecycleAlias> a <AddressAliasType>,
        skos:Concept , owl:NamedIndividual ;
    skos:definition "The address alias has a different lifecycle stage." ;
		rdfs:comment "The address alias has a different lifecycle stage." ;
    skos:inScheme <AddressAliasType> ;
    skos:prefLabel "Lifecycle Alias" .

<AddressAliasType/localeAlias> a <AddressAliasType>,
        skos:Concept , owl:NamedIndividual ;
    skos:definition "The address alias is in a different locale." ;
		rdfs:comment "The address alias is in a different locale." ;
    skos:inScheme <AddressAliasType> ;
    skos:prefLabel "Locale Alias" .

<AddressAliasType/unspecifiedAlias> a <AddressAliasType>,
        skos:Concept , owl:NamedIndividual ;
    skos:definition "The type of address alias is not specified." ;
		rdfs:comment "The type of address alias is not specified." ;
    skos:inScheme <AddressAliasType> ;
    skos:prefLabel "Unspecified Alias" .

<AddressComponentType/addressedObjectIdentifier> a <AddressComponentType>,
        skos:Concept , owl:NamedIndividual ;
    skos:definition "Identifier of the addressed object, e.g. building name or address number." ;
		rdfs:comment "Identifier of the addressed object, e.g. building name or address number." ;
    skos:inScheme <AddressComponentType> ;
    skos:prefLabel "Addressed ObjectIdentifier" .

<AddressComponentType/administrativeAreaName> a <AddressComponentType>,
        skos:Concept , owl:NamedIndividual ;
    skos:definition "Name of an administrative area." ;
		rdfs:comment "Name of an administrative area." ;
    skos:inScheme <AddressComponentType> ;
    skos:prefLabel "Administrative Area Name" .

<AddressComponentType/countryCode> a <AddressComponentType>,
        skos:Concept , owl:NamedIndividual ;
    skos:definition "ISO 3166-1 code for the country, territory or area of geopolitical interest." ;
		rdfs:comment "ISO 3166-1 code for the country, territory or area of geopolitical interest." ;
    skos:inScheme <AddressComponentType> ;
    skos:prefLabel "Country Code" .

<AddressComponentType/countryName> a <AddressComponentType>,
        skos:Concept , owl:NamedIndividual ;
    skos:definition "Name of a country." ;
		rdfs:comment "Name of a country." ;
    skos:inScheme <AddressComponentType> ;
    skos:prefLabel "Country Name" .

<AddressComponentType/localityName> a <AddressComponentType>,
        skos:Concept , owl:NamedIndividual ;
    skos:definition "Name of a locality." ;
		rdfs:comment "Name of a locality." ;
    skos:inScheme <AddressComponentType> ;
    skos:prefLabel "Locality Name" .

<AddressComponentType/postOfficeName> a <AddressComponentType>,
        skos:Concept , owl:NamedIndividual ;
    skos:definition "Name of a post office." ;
		rdfs:comment "Name of a post office." ;
    skos:inScheme <AddressComponentType> ;
    skos:prefLabel "Post Office Name" .

<AddressComponentType/postcode> a <AddressComponentType>,
        skos:Concept , owl:NamedIndividual ;
    skos:definition "Code used for the sorting of mail [SOURCE: UPU S42:2006]." ;
		rdfs:comment "Code used for the sorting of mail [SOURCE: UPU S42:2006]." ;
    skos:inScheme <AddressComponentType> ;
    skos:prefLabel "Postcode" .

<AddressComponentType/thoroughfareName> a <AddressComponentType>,
        skos:Concept , owl:NamedIndividual ;
    skos:definition "Name of a thoroughfare." ;
		rdfs:comment "Name of a thoroughfare." ;
    skos:inScheme <AddressComponentType> ;
    skos:prefLabel "Thoroughfare Name" .

<AddressComponentValueType/abbreviatedAlternative> a <AddressComponentValueType>,
        skos:Concept , owl:NamedIndividual ;
    skos:definition "The alternative component value is an abbreviation." ;
		rdfs:comment "The alternative component value is an abbreviation." ;
    skos:inScheme <AddressComponentValueType> ;
    skos:prefLabel "Abbreviated Alternative" .

<AddressComponentValueType/colloquialAlternative> a <AddressComponentValueType>,
        skos:Concept , owl:NamedIndividual ;
    skos:definition "The alternative component value is a colloquial alternative for the component value." ;
		rdfs:comment "The alternative component value is a colloquial alternative for the component value." ;
    skos:inScheme <AddressComponentValueType> ;
    skos:prefLabel "Colloquial Alternative" .

<AddressComponentValueType/defaultValue> a <AddressComponentValueType>,
        skos:Concept , owl:NamedIndividual ;
    skos:definition "The default component value (i.e. the one that is not an alternative)." ;
		rdfs:comment "The default component value (i.e. the one that is not an alternative)." ;
    skos:inScheme <AddressComponentValueType> ;
    skos:prefLabel "Default Value" .

<AddressComponentValueType/lifecycleAlternative> a <AddressComponentValueType>,
        skos:Concept , owl:NamedIndividual ;
    skos:definition "The alternative component value was used in a different lifecycle stage." ;
		rdfs:comment "The alternative component value was used in a different lifecycle stage." ;
    skos:inScheme <AddressComponentValueType> ;
    skos:prefLabel "Lifecycle Alternative" .

<AddressComponentValueType/localeAlternative> a <AddressComponentValueType>,
        skos:Concept , owl:NamedIndividual ;
    skos:definition "The alternative component value is in a different locale." ;
		rdfs:comment "The alternative component value is in a different locale." ;
    skos:inScheme <AddressComponentValueType> ;
    skos:prefLabel "Locale Alternative" .

<AddressLifecycleStage/current> a <AddressLifecycleStage>,
        skos:Concept , owl:NamedIndividual ;
    skos:definition "The address or address component is currently in use." ;
		rdfs:comment "The address or address component is currently in use." ;
    skos:inScheme <AddressLifecycleStage> ;
    skos:prefLabel "current" .

<AddressLifecycleStage/proposed> a <AddressLifecycleStage>,
        skos:Concept , owl:NamedIndividual ;
    skos:definition "The address or address component has been proposed, i.e. the relevant authority has initiated approval procedures for the use of the address or address component." ;
		rdfs:comment "The address or address component has been proposed, i.e. the relevant authority has initiated approval procedures for the use of the address or address component." ;
    skos:inScheme <AddressLifecycleStage> ;
    skos:prefLabel "proposed" .

<AddressLifecycleStage/rejected> a <AddressLifecycleStage>,
        skos:Concept , owl:NamedIndividual ;
    skos:definition "The address or address component was proposed but rejected." ;
		rdfs:comment "The address or address component was proposed but rejected." ;
    skos:inScheme <AddressLifecycleStage> ;
    skos:prefLabel "rejected" .

<AddressLifecycleStage/reserved> a <AddressLifecycleStage>,
        skos:Concept , owl:NamedIndividual ;
    skos:definition "The address or address component has been reserved for future use." ;
		rdfs:comment "The address or address component has been reserved for future use." ;
    skos:inScheme <AddressLifecycleStage> ;
    skos:prefLabel "reserved" .

<AddressLifecycleStage/retired> a <AddressLifecycleStage>,
        skos:Concept , owl:NamedIndividual ;
    skos:definition "The address or address component was in use at some stage, but not anymore." ;
		rdfs:comment "The address or address component was in use at some stage, but not anymore." ;
    skos:inScheme <AddressLifecycleStage> ;
    skos:prefLabel "retired" .

<AddressLifecycleStage/unknown> a <AddressLifecycleStage>,
        skos:Concept , owl:NamedIndividual ;
    skos:definition "The lifecycle stage of the address or address component is unknown." ;
		rdfs:comment "The lifecycle stage of the address or address component is unknown." ;
    skos:inScheme <AddressLifecycleStage> ;
    skos:prefLabel "unknown" .

<AddressStatus/official> a <AddressStatus>,
        skos:Concept , owl:NamedIndividual ;
    skos:definition "An official addressing authority assigned the address." ;
		rdfs:comment "An official addressing authority assigned the address." ;
    skos:inScheme <AddressStatus> ;
    skos:prefLabel "official" .

<AddressStatus/unknown> a <AddressStatus>,
        skos:Concept , owl:NamedIndividual ;
    skos:definition "The status of the address is unknown." ;
		rdfs:comment "The status of the address is unknown." ;
    skos:inScheme <AddressStatus> ;
    skos:prefLabel "unknown" .

<AddressStatus/unofficial> a <AddressStatus>,
        skos:Concept , owl:NamedIndividual ;
    skos:definition "The address was not assigned by an official addressing authority." ;
		rdfs:comment "The address was not assigned by an official addressing authority." ;
    skos:inScheme <AddressStatus> ;
    skos:prefLabel "unofficial" .

<AddressTypology/area> a <AddressTypology>,
        skos:Concept , owl:NamedIndividual ;
    skos:definition "The address class is based on a division of land or water into demarcated areas, such as neighbourhoods or precincts or cadastral features." ;
		rdfs:comment "The address class is based on a division of land or water into demarcated areas, such as neighbourhoods or precincts or cadastral features." ;
    skos:inScheme <AddressTypology> ;
    skos:prefLabel "area" .

<AddressTypology/service> a <AddressTypology>,
        skos:Concept , owl:NamedIndividual ;
    skos:definition "The address class is based on delivery or collection services, such as a group of post boxes at the same location or poste restante." ;
		rdfs:comment "The address class is based on delivery or collection services, such as a group of post boxes at the same location or poste restante." ;
    skos:inScheme <AddressTypology> ;
    skos:prefLabel "service" .

<AddressTypology/thoroughfare> a <AddressTypology>,
        skos:Concept , owl:NamedIndividual ;
    skos:definition "The address class is based on navigable access features, such as streets or canals." ;
		rdfs:comment "The address class is based on navigable access features, such as streets or canals." ;
    skos:inScheme <AddressTypology> ;
    skos:prefLabel "thoroughfare" .

<AddressableObjectLifecycleStage/approved> a <AddressableObjectLifecycleStage>,
        skos:Concept , owl:NamedIndividual ;
    skos:definition "The establishment or construction of the addressable object has been approved, i.e. the relevant authority has given approval for the establishment or construction of the addressable object." ;
		rdfs:comment "The establishment or construction of the addressable object has been approved, i.e. the relevant authority has given approval for the establishment or construction of the addressable object." ;
    skos:inScheme <AddressableObjectLifecycleStage> ;
    skos:prefLabel "approved" .

<AddressableObjectLifecycleStage/ceasedToExist> a <AddressableObjectLifecycleStage>,
        skos:Concept , owl:NamedIndividual ;
    skos:definition "The addressable object does not exist anymore (e.g. it has been demolished)." ;
		rdfs:comment "The addressable object does not exist anymore (e.g. it has been demolished)." ;
    skos:inScheme <AddressableObjectLifecycleStage> ;
    skos:prefLabel "ceasedToExist" .

<AddressableObjectLifecycleStage/exists> a <AddressableObjectLifecycleStage>,
        skos:Concept , owl:NamedIndividual ;
    skos:definition "The addressable object exists." ;
		rdfs:comment "The addressable object exists." ;
    skos:inScheme <AddressableObjectLifecycleStage> ;
    skos:prefLabel "exists" .

<AddressableObjectLifecycleStage/proposed> a <AddressableObjectLifecycleStage>,
        skos:Concept , owl:NamedIndividual ;
    skos:definition "The establishment or construction of the addressable object has been proposed, i.e. the relevant authority has initiated approval procedures." ;
		rdfs:comment "The establishment or construction of the addressable object has been proposed, i.e. the relevant authority has initiated approval procedures." ;
    skos:inScheme <AddressableObjectLifecycleStage> ;
    skos:prefLabel "proposed" .

<AddressableObjectLifecycleStage/underConstruction> a <AddressableObjectLifecycleStage>,
        skos:Concept , owl:NamedIndividual ;
    skos:definition "The establishment or construction of the addressable object is in progress." ;
		rdfs:comment "The establishment or construction of the addressable object is in progress." ;
    skos:inScheme <AddressableObjectLifecycleStage> ;
    skos:prefLabel "underConstruction" .

<AddressableObjectLifecycleStage/unknown> a <AddressableObjectLifecycleStage>,
        skos:Concept , owl:NamedIndividual ;
    skos:definition "The lifecycle stage of the addressable object is unknown." ;
		rdfs:comment "The lifecycle stage of the addressable object is unknown." ;
    skos:inScheme <AddressableObjectLifecycleStage> ;
    skos:prefLabel "unknown" .

<AddressStatus> a skos:ConceptScheme ;
    skos:prefLabel "AddressStatus - ConceptScheme" .

<AddressTypology> a skos:ConceptScheme ;
    skos:prefLabel "Address Typology - ConceptScheme" .

<AddressAliasType> a skos:ConceptScheme ;
    skos:prefLabel "Address Alias Type - ConceptScheme" .

<AddressComponentValueType> a skos:ConceptScheme ;
    skos:prefLabel "Address Component Value Type - ConceptScheme" .

<AddressLifecycleStage> a skos:ConceptScheme ;
    skos:prefLabel "Address Lifecycle Stage - ConceptScheme" .

<AddressableObjectLifecycleStage> a skos:ConceptScheme ;
    skos:prefLabel "Addressable Object Lifecycle Stage - ConceptScheme" .

<AddressComponentType> a skos:ConceptScheme ;
    skos:prefLabel "Address ComponentType - ConceptScheme" .
